minuska/theories/default_static_model.v
@@ -1,7 +1,6 @@
 From Minuska Require Import
     prelude
-    spec_syntax
-    spec_semantics
+    spec
     string_variables
 .
 
