minuska/theories/lowlang.v
@@ -1,0 +1,1570 @@
+From Minuska Require Import
+    prelude
+    spec
+.
+
+
+
+
+#[universes(polymorphic=yes, cumulative=yes)]
+Inductive PreTerm' (operator : Type) (operand : Type)
+: Type
+:=
+| pt_operator (s : operator)
+| pt_app_operand
+    (aps : PreTerm' operator operand)
+    (b : operand) 
+| pt_app_ao
+    (aps : PreTerm' operator operand)
+    (x : PreTerm' operator operand)
+.
+
+
+#[universes(polymorphic=yes, cumulative=yes)]
+Variant Term'
+    (Operator : Type)
+    (Operand : Type)
+    : Type :=
+| term_preterm (ao : PreTerm' Operator Operand)
+| term_operand (operand : Operand)
+.
+
+
+Arguments term_operand {Operator Operand}%_type_scope operand.
+Arguments term_preterm {Operator Operand}%_type_scope ao.
+
+Arguments pt_operator {operator operand}%_type_scope s.
+Arguments pt_app_operand {operator operand}%_type_scope aps b.
+Arguments pt_app_ao {operator operand}%_type_scope aps x.
+
+Definition GroundTerm {Σ : StaticModel}
+    := Term' symbol builtin_value
+.
+
+Inductive Expression
+    {Σ : StaticModel}
+    :=
+| ft_element (e : GroundTerm)
+| ft_variable (x : variable)
+| ft_nullary (f : builtin_nullary_function)
+| ft_unary (f : builtin_unary_function) (t : Expression)
+| ft_binary (f : builtin_binary_function) (t1 : Expression) (t2 : Expression)
+| ft_ternary (f : builtin_ternary_function) (t1 : Expression) (t2 : Expression) (t3 : Expression)
+.
+
+
+Inductive AtomicProposition {Σ : StaticModel} :=
+| apeq (e1 : Expression) (e2 : Expression)
+.
+
+
+Definition SymbolicTerm {Σ : StaticModel}
+    := Term' symbol BuiltinOrVar
+.
+
+Inductive SideCondition {Σ : StaticModel} :=
+| sc_constraint (c : AtomicProposition)
+.
+
+Definition ExpressionTerm {Σ : StaticModel} :=
+    Term' symbol Expression
+.
+
+
+Inductive LeftRight : Set := LR_Left | LR_Right.
+
+Record RewritingRule
+    {Σ : StaticModel}
+    (Act : Set)
+:= mkRewritingRule
+{
+    fr_from : SymbolicTerm ;
+    fr_to : ExpressionTerm ;
+    fr_scs : list SideCondition ;
+    fr_act : Act ;
+}.
+
+Arguments fr_from {Σ} {Act}%_type_scope r.
+Arguments fr_to {Σ} {Act}%_type_scope r.
+Arguments fr_scs {Σ} {Act}%_type_scope r.
+Arguments fr_act {Σ} {Act}%_type_scope r.
+
+Definition RewritingTheory
+    {Σ : StaticModel}
+    (Act : Set)
+    := list (RewritingRule Act)
+.
+
+
+Definition to_Term'
+    {Σ : StaticModel}
+    {T : Type}
+    (x : ((T)+(PreTerm' symbol T)))
+    : Term' symbol T
+:=
+match x with
+| inl x' => term_operand x'
+| inr x' => term_preterm x'
+end
+.
+
+Definition helper {Σ : StaticModel} {T : Type} a b : PreTerm' symbol T
+    :=match b with
+            | term_operand b' => pt_app_operand a b'
+            | term_preterm b' => pt_app_ao a b'
+            end.
+
+Definition to_PreTerm'
+    {Σ : StaticModel}
+    {T : Type}
+    (s : symbol)
+    (l : list ((Term' symbol T)))
+    : PreTerm' symbol T
+:=
+    fold_left
+        helper
+        l
+        (pt_operator s)
+.
+
+Lemma to_PreTerm'_app
+    {Σ : StaticModel}
+    {T : Type}
+    (s : symbol)
+    (l1 l2 : list ((Term' symbol T)))
+    : to_PreTerm' s (l1 ++ l2) = fold_left helper l2 (to_PreTerm' s l1)
+.
+Proof.
+    unfold to_PreTerm'.
+    rewrite fold_left_app.
+    reflexivity.
+Qed.
+
+Definition apply_symbol'
+    {Σ : StaticModel}
+    {T : Type}
+    (s : symbol)
+: 
+    list ((Term' symbol T)) ->
+    Term' symbol T
+:=
+    fun l =>
+    (to_Term' (inr (to_PreTerm' ((s):symbol) l)))
+.
+
+Definition to_Term''
+    {T0 : Type}
+    {T : Type}
+    (x : ((T)+(PreTerm' T0 T)))
+    : Term' T0 T
+:=
+match x with
+| inl x' => term_operand x'
+| inr x' => term_preterm x'
+end
+.
+
+Definition helper'' {T0 : Type} {T : Type} a b : PreTerm' T0 T
+    :=match b with
+            | term_operand b' => pt_app_operand a b'
+            | term_preterm b' => pt_app_ao a b'
+            end.
+
+
+Definition to_PreTerm''
+    {T0 : Type}
+    {T : Type}
+    (s : T0)
+    (l : list ((Term' T0 T)))
+    : PreTerm' T0 T
+:=
+    fold_left
+        helper''
+        l
+        (pt_operator s)
+.
+
+
+Definition apply_symbol''
+    {T0 : Type}
+    {T : Type}
+    (s : T0)
+: 
+    list ((Term' T0 T)) ->
+    Term' T0 T
+:=
+    fun l =>
+    (to_Term'' (inr (to_PreTerm'' ((s):T0) l)))
+.
+
+
+
+Fixpoint uglify'
+    {T : Type}
+    {A : Type}
+    (t : @TermOver' T A)
+    {struct t}
+    : Term' T A
+:=
+    match t with
+    | t_over a => term_operand a
+    | t_term s l => apply_symbol'' s (map uglify' l)
+    end
+.
+
+Fixpoint PreTerm'_get_symbol
+    {T : Type}
+    {A : Type}
+    (pt : PreTerm' T A)
+    : T
+:=
+    match pt with
+    | pt_operator s => s
+    | pt_app_operand x y => PreTerm'_get_symbol x
+    | pt_app_ao x y => PreTerm'_get_symbol x
+    end
+.
+
+Fixpoint prettify'
+    {T : Type}
+    {A : Type}
+    (pt : PreTerm' T A)
+    : @TermOver' T A
+:=
+    t_term
+        (PreTerm'_get_symbol pt) (
+        ((fix go (pt : PreTerm' T A) : list (@TermOver' T A) :=
+            match pt with
+            | pt_operator _ => []
+            | pt_app_operand x y => (go x)++[(t_over y)]
+            | pt_app_ao x y => (go x)++[(prettify' y)]
+            end
+        ) pt))
+.
+
+Definition prettify
+    {T : Type}
+    {A : Type}
+    (t : Term' T A)
+    : ((@TermOver' T A))
+:=
+    match t with
+    | term_preterm pt => (prettify' pt)
+    | term_operand a => t_over a
+    end
+.
+
+Lemma to_PreTerm''_app
+    {T0 : Type}
+    {T : Type}
+    (s : T0)
+    (l1 l2 : list ((Term' T0 T)))
+    : to_PreTerm'' s (l1 ++ l2) = fold_left helper'' l2 (to_PreTerm'' s l1)
+.
+Proof.
+    unfold to_PreTerm''.
+    rewrite fold_left_app.
+    reflexivity.
+Qed.
+
+
+#[global]
+Instance cancel_prettify_uglify
+    {T : Type}
+    {A : Type}
+    : Cancel eq (@prettify T A) (@uglify' T A)
+.
+Proof.
+    intros x.
+    induction x.
+    {
+        simpl. reflexivity.
+    }
+    {
+        simpl.
+
+        revert s H.
+        induction l using rev_ind; intros s H; simpl.
+        {
+            reflexivity.
+        }
+        {
+            assert (Hs: (PreTerm'_get_symbol (to_PreTerm'' s (map uglify' l))) = s).
+            {
+                clear.
+                induction l using rev_ind; simpl.
+                { reflexivity. }
+                {
+                    unfold to_PreTerm''. simpl.
+                    rewrite map_app. simpl.
+                    rewrite fold_left_app. simpl.
+                    destruct (uglify' x); apply IHl.
+                }
+            }
+
+            apply Forall_app in H. destruct H as [H2 H1]. (*
+            apply Forall_inv in H as H1.
+            apply Forall_inv_tail in H as H2.*)
+            specialize (IHl s H2).
+            simpl.
+            unfold helper.
+            rewrite map_app.
+            rewrite to_PreTerm''_app.
+            simpl.
+            unfold helper.
+            destruct (uglify' x) eqn:Hux.
+            {
+                simpl.
+                remember ((to_PreTerm'' s (map uglify' l)) ) as tpt.
+                destruct tpt; simpl in *.
+                {
+                    inversion IHl; subst; clear IHl.
+                    simpl in *.
+                    apply Forall_inv in H1.
+                    clear H0.
+                    rewrite Hux in H1. simpl in H1.
+                    subst x.
+                    reflexivity.
+                }
+                {
+                    simpl in *.
+                    f_equal.
+                    {
+                        apply Hs.
+                    }
+                    {
+                        inversion IHl; subst; clear IHl.
+                        clear H0.
+                        inversion H1; subst; clear H1. clear H4.
+                        rewrite Hux in H3. simpl in H3. subst x.
+                        reflexivity.
+                    }
+                }
+                {
+                    simpl in *.
+                    f_equal.
+                    {
+                        apply Hs.
+                    }
+                    {
+                        inversion IHl; subst; clear IHl.
+                        clear H0.
+                        inversion H1; subst; clear H1. clear H4.
+                        rewrite Hux in H3. simpl in H3. subst x.
+                        reflexivity.
+                    }
+                }
+            }
+            {
+                simpl.
+                remember ((to_PreTerm'' s (map uglify' l)) ) as tpt.
+                destruct tpt; simpl in *.
+                {
+                    inversion IHl; subst; clear IHl.
+                    simpl in *.
+                    apply Forall_inv in H1.
+                    clear H0.
+                    rewrite Hux in H1. simpl in H1.
+                    subst x.
+                    reflexivity.
+                }
+                {
+                    simpl in *.
+                    f_equal.
+                    {
+                        apply Hs.
+                    }
+                    {
+                        inversion IHl; subst; clear IHl.
+                        clear H0.
+                        inversion H1; subst; clear H1. clear H4.
+                        rewrite Hux in H3. simpl in H3. subst x.
+                        reflexivity.
+                    }
+                }
+                {
+                    simpl in *.
+                    f_equal.
+                    {
+                        apply Hs.
+                    }
+                    {
+                        inversion IHl; subst; clear IHl.
+                        clear H0.
+                        inversion H1; subst; clear H1. clear H4.
+                        rewrite Hux in H3. simpl in H3. subst x.
+                        reflexivity.
+                    }
+                }
+            }
+        }
+    }
+Qed.
+
+
+
+#[global]
+Instance cancel_uglify_prettify
+    {T : Type}
+    {A : Type}
+    : Cancel eq (@uglify' T A) (@prettify T A)
+.
+Proof.
+    intros x.
+    destruct x; simpl.
+    {
+        induction ao; simpl.
+        {
+            reflexivity.
+        }
+        {
+            unfold apply_symbol''. simpl. f_equal.
+            unfold to_PreTerm''.
+            rewrite map_app.
+            rewrite fold_left_app.
+            simpl.
+            f_equal.
+            revert IHao.
+            induction ao; intros IHao'.
+            {
+                simpl. reflexivity.
+            }
+            {
+                simpl in *.
+                unfold apply_symbol'' in *. simpl in *.
+                inversion IHao'; subst; clear IHao'.
+                unfold to_PreTerm'' in *.
+                rewrite map_app in H0.
+                rewrite fold_left_app in H0.
+                simpl in H0.
+                inversion H0; subst; clear H0.
+                simpl.
+                rewrite H1.
+                reflexivity.
+            }
+            {
+                simpl in *.
+                unfold apply_symbol'' in *. simpl in *.
+                inversion IHao'; subst; clear IHao'.
+                unfold to_PreTerm'' in *.
+                rewrite map_app in H0.
+                rewrite fold_left_app in H0.
+                simpl in H0.
+                inversion H0; subst; clear H0.
+                simpl.
+                reflexivity.
+            }
+        }
+        {
+            unfold apply_symbol''. simpl. f_equal.
+            unfold to_PreTerm''.
+            rewrite map_app.
+            rewrite fold_left_app.
+            simpl.
+            rewrite IHao2.
+            simpl.
+            f_equal.
+
+
+            revert IHao1 IHao2.
+            induction ao1; intros IHao1' IHao2'.
+            {
+                simpl. reflexivity.
+            }
+            {
+                simpl in *.
+                unfold apply_symbol'' in *. simpl in *.
+                inversion IHao1'; subst; clear IHao1'.
+                unfold to_PreTerm'' in *.
+                rewrite map_app in H0.
+                rewrite fold_left_app in H0.
+                simpl in H0.
+                inversion H0; subst; clear H0.
+                simpl.
+                rewrite H1.
+                reflexivity.
+            }
+            {
+                simpl in *.
+                unfold apply_symbol'' in *. simpl in *.
+                inversion IHao1'; subst; clear IHao1'.
+                unfold to_PreTerm'' in *.
+                rewrite map_app in H0.
+                rewrite fold_left_app in H0.
+                simpl in H0.
+                inversion H0; subst; clear H0.
+                simpl.
+                reflexivity.
+            }
+        }
+    }
+    {
+        reflexivity.
+    }
+Qed.
+
+
+Lemma uglify'_prettify'
+    {Σ : StaticModel}
+    {T : Type}
+    (t : PreTerm' symbol T)
+    :
+    uglify' (prettify' t) = term_preterm t
+.
+Proof.
+    rewrite <- (cancel uglify' prettify (term_preterm t)).
+    apply f_equal.
+    simpl. reflexivity.
+Qed.
+
+
+Definition BoV_to_Expr
+    {Σ : StaticModel}
+    (bov : BuiltinOrVar)
+    : Expression
+:=
+    match bov with
+    | bov_builtin b => (ft_element (uglify' (t_over b)))
+    | bov_variable x => ft_variable x
+    end
+.
+
+Definition TermOverBoV_to_TermOverExpr
+    {Σ : StaticModel}
+    (t : TermOver BuiltinOrVar)
+    : TermOver Expression
+:=
+    TermOver_map BoV_to_Expr t
+.
+
+
+Fixpoint Expression_subst
+    {Σ : StaticModel}
+    (e : Expression)
+    (x : variable)
+    (e' : Expression)
+    : Expression
+:=    
+match e with
+| ft_element g => ft_element g
+| ft_variable y =>
+    if (decide (y = x)) then e' else (ft_variable y)
+| ft_nullary f => ft_nullary f
+| ft_unary f e1 => ft_unary f (Expression_subst e1 x e')
+| ft_binary f e1 e2 => ft_binary f (Expression_subst e1 x e') (Expression_subst e2 x e')
+| ft_ternary f e1 e2 e3 => ft_ternary f (Expression_subst e1 x e') (Expression_subst e2 x e') (Expression_subst e3 x e')
+end
+.
+
+
+Fixpoint Expression2_to_Expression
+    {Σ : StaticModel}
+    (e : Expression2)
+    : Expression
+:=
+match e with
+| e_ground g => ft_element (uglify' g)
+| e_variable x => ft_variable x
+| e_nullary f => ft_nullary f
+| e_unary f e1 => ft_unary f (Expression2_to_Expression e1)
+| e_binary f e1 e2 => ft_binary f (Expression2_to_Expression e1) (Expression2_to_Expression e2)
+| e_ternary f e1 e2 e3 => ft_ternary f (Expression2_to_Expression e1) (Expression2_to_Expression e2) (Expression2_to_Expression e3)
+end
+.
+
+
+Fixpoint Expression_to_Expression2
+    {Σ : StaticModel}
+    (e : Expression)
+    : Expression2
+:=
+match e with
+| ft_element g => e_ground (prettify g)
+| ft_variable x => e_variable x
+| ft_nullary f => e_nullary f
+| ft_unary f e1 => e_unary f (Expression_to_Expression2 e1)
+| ft_binary f e1 e2 => e_binary f (Expression_to_Expression2 e1) (Expression_to_Expression2 e2)
+| ft_ternary f e1 e2 e3 => e_ternary f (Expression_to_Expression2 e1) (Expression_to_Expression2 e2) (Expression_to_Expression2 e3)
+end
+.
+
+#[export]
+Instance cancel_expression_expression2
+    {Σ : StaticModel}
+    : Cancel eq Expression2_to_Expression Expression_to_Expression2
+.
+Proof.
+    intros e.
+    induction e; simpl; (repeat (rewrite (cancel uglify' prettify))); ltac1:(congruence).
+Qed.
+
+#[export]
+Instance cancel_expression2_expression
+    {Σ : StaticModel}
+    : Cancel eq Expression_to_Expression2 Expression2_to_Expression
+.
+Proof.
+    intros e.
+    induction e; simpl; (repeat (rewrite (cancel prettify uglify'))); ltac1:(congruence).
+Qed.
+
+
+
+Definition sc2_to_sc
+    {Σ : StaticModel}
+    (c : SideCondition2)
+    : SideCondition
+.
+Proof.
+    constructor.
+    constructor.
+    { exact (Expression2_to_Expression (sc_left c)). }
+    { exact (Expression2_to_Expression (sc_right c)). }
+Defined.
+
+Definition sc_to_sc2
+    {Σ : StaticModel}
+    (c : SideCondition)
+    : SideCondition2
+.
+Proof.
+    destruct c.
+    destruct c.
+    constructor.
+    {
+        apply Expression_to_Expression2. exact e1.
+    }
+    {
+        apply Expression_to_Expression2. exact e2.
+    }
+Defined.
+
+#[export]
+Instance cancel_sc_sc2
+    {Σ : StaticModel}
+    :
+    Cancel eq (sc_to_sc2) (sc2_to_sc)
+.
+Proof.
+    intros c; destruct c; simpl.
+    rewrite (cancel Expression_to_Expression2 Expression2_to_Expression).
+    rewrite (cancel Expression_to_Expression2 Expression2_to_Expression).
+    reflexivity.
+Qed.
+
+#[export]
+Instance cancel_sc2_sc
+    {Σ : StaticModel}
+    :
+    Cancel eq (sc2_to_sc) (sc_to_sc2)
+.
+Proof.
+    intros c. destruct c; destruct c; simpl.
+    unfold sc2_to_sc. simpl.
+    rewrite (cancel Expression2_to_Expression Expression_to_Expression2).
+    rewrite (cancel Expression2_to_Expression Expression_to_Expression2).
+    reflexivity.
+Qed.
+
+
+Definition r_to_fr
+    {Σ : StaticModel}
+    {Act : Set}
+    (r : RewritingRule2 Act)
+    : RewritingRule Act
+:=
+    mkRewritingRule
+        Σ
+        Act
+        (uglify' (r_from r))
+        (uglify' (TermOver_map Expression2_to_Expression (r_to r)))
+        (fmap sc2_to_sc (r_scs r))
+        (r_act r)
+.
+
+Definition fr_to_r
+    {Σ : StaticModel}
+    {Act : Set}
+    (r : RewritingRule Act)
+    : RewritingRule2 Act
+.
+Proof.
+    destruct r.
+    constructor.
+    { exact (prettify fr_from0). }
+    { 
+        apply prettify in fr_to0.
+        apply (TermOver_map Expression_to_Expression2).
+        exact fr_to0.
+    }
+    {
+        apply (fmap sc_to_sc2).
+        exact fr_scs0.
+    }
+    {
+        exact fr_act0.
+    }
+Defined.
+
+
+#[export]
+Instance cancel_TermOver_map
+    {Σ : StaticModel}
+    (A B : Type)
+    (f : A -> B)
+    (g : B -> A)
+    :
+    Cancel eq f g ->
+    Cancel eq (TermOver_map f) (TermOver_map g)
+.
+Proof.
+    intros Hcancel.
+    intros t.
+    induction t; simpl.
+    { rewrite (cancel f g). reflexivity. }
+    {
+        f_equal.
+        induction l; simpl.
+        { reflexivity. }
+        {
+            rewrite Forall_cons in H.
+            destruct H as [H1 H2].
+            specialize (IHl H2).
+            rewrite H1. rewrite IHl.
+            reflexivity.
+        }
+    }
+Qed.
+
+
+
+Definition Valuation {Σ : StaticModel}
+        := gmap variable GroundTerm
+    .
+
+#[export]
+Instance VarsOf_valuation
+    {Σ : StaticModel}
+    {var : Type}
+    {_varED : EqDecision var}
+    {_varCnt : Countable var}
+    : VarsOf (gmap var GroundTerm) var
+:= {|
+    vars_of := fun ρ => dom ρ ; 
+|}.
+
+
+Fixpoint Expression_evaluate
+    {Σ : StaticModel}
+    (ρ : gmap variable GroundTerm)
+    (t : Expression)
+    : option GroundTerm :=
+match t with
+| ft_element e => Some e
+| ft_variable x => ρ !! x
+| ft_nullary f =>
+    Some (uglify' (builtin_nullary_function_interp f))
+| ft_unary f t =>
+    e ← prettify <$> Expression_evaluate ρ t;
+    Some (uglify' (builtin_unary_function_interp f e))
+| ft_binary f t1 t2 =>
+    e1 ← prettify <$> Expression_evaluate ρ t1;
+    e2 ← prettify <$> Expression_evaluate ρ t2;
+    Some (uglify' (builtin_binary_function_interp f e1 e2))
+| ft_ternary f t1 t2 t3 =>
+    e1 ← prettify <$> Expression_evaluate ρ t1;
+    e2 ← prettify <$> Expression_evaluate ρ t2;
+    e3 ← prettify <$> Expression_evaluate ρ t3;
+    Some (uglify' (builtin_ternary_function_interp f e1 e2 e3))
+end.
+
+
+Definition val_satisfies_ap
+    {Σ : StaticModel} (ρ : Valuation) (ap : AtomicProposition)
+    : Type :=
+match ap with
+| apeq e1 e2 => 
+    let v1 := Expression_evaluate ρ e1 in
+    let v2 := Expression_evaluate ρ e2 in
+    v1 = v2 /\ isSome v1
+end
+.
+
+#[export]
+Program Instance Satisfies_val_ap
+    {Σ : StaticModel} :
+    Satisfies
+        (gmap variable GroundTerm)
+        unit
+        AtomicProposition
+        variable
+:= {|
+    satisfies := fun ρ u ap => val_satisfies_ap ρ ap ;
+|}.
+
+
+Inductive aoxy_satisfies_aoxz
+    {Σ : StaticModel}
+    {V X Y Z var : Type}
+    {_varED : EqDecision var}
+    {_varCnt : Countable var}
+    {_VV : VarsOf V var}
+    {_SV : SubsetEq V}
+    {_S1 : Satisfies V (Y) Z var}
+    {_S2 : Satisfies V (Y) (PreTerm' X Z) var}
+    {_S3 : Satisfies V ((PreTerm' X Y)) Z var}
+
+    :
+    V ->
+    ((PreTerm' X Y)) ->
+    PreTerm' X Z ->
+    Type :=
+
+| asa_x:
+    forall ρ x,
+        aoxy_satisfies_aoxz
+            ρ
+            (@pt_operator X Y x)
+            (@pt_operator X Z x)
+
+| asa_operand:
+    forall ρ aoxy aoxz y z,
+        aoxy_satisfies_aoxz ρ aoxy aoxz ->
+        satisfies ρ y z ->
+        aoxy_satisfies_aoxz
+            ρ
+            (pt_app_operand aoxy y)
+            (pt_app_operand aoxz z)
+
+| asa_operand_asa:
+    forall ρ aoxy aoxz aoxy2 z,
+        aoxy_satisfies_aoxz ρ aoxy aoxz ->
+        satisfies ρ aoxy2 z ->
+        aoxy_satisfies_aoxz
+        (* The right-side, the symbolic one, has more compact representation - so *)
+            ρ
+            (pt_app_ao aoxy aoxy2)
+            (pt_app_operand aoxz z)
+
+| asa_asa_operand:
+    forall
+        (ρ : V)
+        (aoxy : PreTerm' X Y)
+        (aoxz aoxz2 : PreTerm' X Z)
+        (y : Y),
+        aoxy_satisfies_aoxz ρ aoxy aoxz ->
+        satisfies ρ y aoxz2 ->
+        aoxy_satisfies_aoxz
+            ρ
+            (pt_app_operand aoxy y)
+            ((pt_app_ao aoxz aoxz2))
+
+| asa_asa:
+    forall ρ aoxy1 aoxy2 aoxz1 aoxz2,
+        aoxy_satisfies_aoxz ρ aoxy1 aoxz1 ->
+        aoxy_satisfies_aoxz ρ aoxy2 aoxz2 ->
+        aoxy_satisfies_aoxz
+            ρ
+            (pt_app_ao aoxy1 aoxy2)
+            (pt_app_ao aoxz1 aoxz2)
+.
+
+
+#[export]
+Instance Satisfies_aoxy_aoxz
+    {Σ : StaticModel}
+    {V X Y Z var : Type}
+    {_varED : EqDecision var}
+    {_varCnt : Countable var}
+    {_VV : VarsOf V var}
+    {_SV : SubsetEq V}
+    {_S1 : Satisfies V (Y) Z var}
+    {_S2 : Satisfies V (Y) (PreTerm' X Z) var}
+    {_S3 : Satisfies V ((PreTerm' X Y)) Z var}
+    :
+    Satisfies V ((PreTerm' X Y)) (PreTerm' X Z) var
+:= {|
+    satisfies := aoxy_satisfies_aoxz ;
+|}.
+
+
+Inductive aoxyo_satisfies_aoxzo
+    {Σ : StaticModel}
+    (V X Y Z var : Type)
+    {_varED : EqDecision var}
+    {_varCnt : Countable var}
+    {_VV : VarsOf V var}
+    {_SV : SubsetEq V}
+    {_S1 : Satisfies V Y Z var}
+    {_S2 : Satisfies V ((PreTerm' X Y)) Z var}
+    {_S3 : Satisfies V ((PreTerm' X Y)) (PreTerm' X Z) var}
+    : V ->
+        ((Term' X Y)) ->
+        (Term' X Z) ->
+        Type
+:=
+| axysaxz_app:
+    forall
+        (ρ : V)
+        (xy : PreTerm' X Y)
+        (xz : PreTerm' X Z)
+        (pf : satisfies ρ xy xz),
+        aoxyo_satisfies_aoxzo V X Y Z var ρ (@term_preterm _ _  xy) (term_preterm xz)
+
+| axysaxz_operand:
+    forall (ρ : V) (y : Y) (z : Z) (pf : satisfies ρ y z),
+        aoxyo_satisfies_aoxzo V X Y Z var ρ (@term_operand X Y y) (@term_operand X Z z)
+
+| axysaxz_combined:
+    forall (ρ : V) axy axz,
+        satisfies ρ axy axz ->
+        aoxyo_satisfies_aoxzo V X Y Z var ρ (@term_preterm _ _  axy) (@term_operand X Z axz)
+.
+
+#[export]
+Program Instance Satisfies_aoxyo_aoxzo
+    {Σ : StaticModel}
+    (V X Y Z var : Type)
+    {_varED : EqDecision var}
+    {_varCnt : Countable var}
+    {_VV : VarsOf V var}
+    {_SV : SubsetEq V}
+    {_S1 : Satisfies V Y Z var}
+    {_S2 : Satisfies V ((PreTerm' X Y)) Z var}
+    {_S3 : Satisfies V ((PreTerm' X Y)) (PreTerm' X Z) var}
+    :
+    Satisfies V ((Term' X Y)) (Term' X Z) var
+:= {|
+    satisfies := aoxyo_satisfies_aoxzo V X Y Z var;
+|}.
+
+Inductive builtin_satisfies_BuiltinOrVar
+    {Σ : StaticModel}
+    (ρ : Valuation)
+    :
+    builtin_value ->
+    BuiltinOrVar ->
+    Type :=
+
+| bsbv_builtin:
+    forall b,
+        builtin_satisfies_BuiltinOrVar ρ b (bov_builtin b)
+
+| bsbv_var:
+    forall (b : builtin_value) (x : variable),
+        ρ !! x = Some (@term_operand symbol builtin_value b) ->
+        builtin_satisfies_BuiltinOrVar ρ b (bov_variable x)
+.
+
+Definition builtin_satisfies_BuiltinOrVar'
+    {Σ : StaticModel}
+    (ρ : Valuation)
+    (b : builtin_value)
+    (bov : BuiltinOrVar)
+    : Type
+:= builtin_satisfies_BuiltinOrVar ρ b bov.
+
+#[export]
+Instance Subseteq_Valuation {Σ : StaticModel}
+    : SubsetEq Valuation
+.
+Proof.
+    unfold Valuation.
+    apply _.
+Defined.
+
+
+
+#[export]
+Instance Satisfies_builtin_BuiltinOrVar
+    {Σ : StaticModel}
+    :
+    Satisfies Valuation (builtin_value) BuiltinOrVar variable
+:= {|
+    satisfies := builtin_satisfies_BuiltinOrVar' ;
+|}.
+
+Definition PreTerm'_symbol_builtin_satisfies_BuiltinOrVar
+    {Σ : StaticModel}
+    (ρ : Valuation)
+    (aop : PreTerm' symbol builtin_value)
+    (bov : BuiltinOrVar)
+    : Type :=
+match bov with
+| bov_builtin _ => False
+| bov_variable x => ρ !! x = Some (term_preterm aop)
+end.
+
+#[export]
+Program Instance Satisfies__PreTerm'_symbol_builtin__BuiltinOrVar
+    {Σ : StaticModel}
+    : Satisfies Valuation ((PreTerm' symbol builtin_value)) BuiltinOrVar variable
+:= {| 
+    satisfies := PreTerm'_symbol_builtin_satisfies_BuiltinOrVar
+|}.
+
+Definition PreTerm'_symbol_builtin_satisfies'_BuiltinOrVar
+    {Σ : StaticModel}
+    (ρ : Valuation)
+    (aop : (PreTerm' symbol builtin_value))
+    (bov : BuiltinOrVar)
+    : Type
+:= PreTerm'_symbol_builtin_satisfies_BuiltinOrVar ρ aop bov.
+
+#[export]
+Instance Satisfies_PreTerm'_symbol_builtin_BuiltinOrVar
+    {Σ : StaticModel}
+    :
+    Satisfies Valuation ((PreTerm' symbol builtin_value)) BuiltinOrVar variable
+:= {|
+    satisfies := PreTerm'_symbol_builtin_satisfies'_BuiltinOrVar ;
+|}.
+
+
+
+#[export]
+Instance Satisfies__builtin__ao'B
+    {Σ : StaticModel}
+    {V B var : Type}
+    {_SV : SubsetEq V}
+    {_EDv : EqDecision var}
+    {_Cv : Countable var}
+    {_VV : VarsOf V var}
+    :
+    Satisfies
+        V
+        (builtin_value)
+        (PreTerm' symbol B)
+        var
+:= {| 
+    satisfies := fun _ _ _ => false ;
+|}.
+
+
+
+#[export]
+Instance Satisfies_aos__builtin_BuiltinOrVar
+    {Σ : StaticModel}
+    :
+    Satisfies
+        Valuation
+        ((PreTerm' symbol builtin_value))
+        (PreTerm' symbol BuiltinOrVar)
+        variable
+.
+Proof.
+    apply @Satisfies_aoxy_aoxz.
+    {
+        apply _.
+    }
+    {
+        apply Satisfies__builtin__ao'B.
+    }
+    {
+        apply _.
+    }
+Defined.
+
+
+#[export]
+Instance Satisfies_aosb_aosbf
+    {Σ : StaticModel}
+    {A B : Type}
+    {SatAB : Satisfies Valuation (A) B variable}
+    {_S2 : Satisfies Valuation (A) (PreTerm' symbol B) variable}
+    {SatA'B : Satisfies Valuation ((PreTerm' symbol A)) B variable}
+    :
+    Satisfies Valuation ((PreTerm' symbol A)) (PreTerm' symbol B) variable
+.
+Proof.
+    apply _.
+Defined.
+
+#[export]
+Instance
+Satisfies_aoosb_aoosbf
+    {Σ : StaticModel}
+    :
+    Satisfies
+        Valuation
+        ((Term' symbol builtin_value))
+        (Term' symbol BuiltinOrVar)
+        variable
+.
+Proof. apply _. Defined.
+
+#[export]
+Instance Satisfies_valGroundTerm_SymbolicTerm
+    {Σ : StaticModel}
+    :
+    Satisfies
+        Valuation
+        GroundTerm
+        SymbolicTerm
+        variable
+.
+Proof. 
+    apply _.
+Defined.
+
+
+
+
+Definition valuation_satisfies_sc
+    {Σ : StaticModel}
+    (ρ : Valuation)
+    (sc : SideCondition) : Type :=
+match sc with
+| sc_constraint c => satisfies ρ () c
+end.
+
+#[export]
+Instance Satisfies_val_sc
+    {Σ : StaticModel}
+    :
+    Satisfies
+        Valuation
+        unit
+        SideCondition
+        variable
+:= {|
+    satisfies := fun a b c => valuation_satisfies_sc a c ;
+|}.
+
+
+Definition GroundTerm_satisfies_BuiltinOrVar
+    {Σ : StaticModel}
+    (ρ : Valuation)
+    (g : GroundTerm)
+    (bov : BuiltinOrVar)
+    : Type :=
+match bov with
+| bov_builtin b =>
+    match g with
+    | term_preterm _ => False
+    | term_operand b' => b = b'
+    end
+| bov_variable x => ρ !! x = Some g
+end.
+
+#[export]
+Instance Satisfies_GroundTerm_BuiltinOrVar
+    {Σ : StaticModel}
+    :
+    Satisfies Valuation (GroundTerm) BuiltinOrVar variable
+:= {|
+    satisfies := GroundTerm_satisfies_BuiltinOrVar ;
+|}.
+
+
+Definition builtin_value_satisfies_SymbolicTerm
+    {Σ : StaticModel}
+    :
+    Valuation ->
+    builtin_value ->
+    SymbolicTerm ->
+    Type := fun ρ b t =>
+match t with
+| term_preterm _ => False
+| term_operand bov =>
+    satisfies ρ b bov
+end.
+
+#[export]
+Instance Satisfies_builtin_value_SymbolicTerm
+    {Σ : StaticModel}
+    :
+    Satisfies
+        Valuation
+        builtin_value
+        SymbolicTerm
+        variable
+:= {|
+    satisfies :=  builtin_value_satisfies_SymbolicTerm ;
+|}.
+
+Definition PreTerm'_symbol_builtin_value_satisfies_BOV
+    {Σ : StaticModel}
+    (ρ : Valuation)
+    (ao : (PreTerm' symbol builtin_value))
+    (bov : BuiltinOrVar)
+    : Type
+:=
+match bov with
+| bov_builtin _ => False
+| bov_variable x => ρ !! x = Some (term_preterm ao) 
+end
+.
+
+#[export]
+Instance Satisfies__PreTerm'_symbol_builtin_value__BOV
+    {Σ : StaticModel}
+    {V : Type}
+    :
+    Satisfies
+        Valuation
+        ((PreTerm' symbol builtin_value))
+        BuiltinOrVar
+        variable
+:= {|
+    satisfies := PreTerm'_symbol_builtin_value_satisfies_BOV;
+|}.
+
+Definition PreTerm'_symbol_A_satisfies_SymbolicTermB'
+    {Σ : StaticModel}
+    (V A B var : Type)
+    {_varED : EqDecision var}
+    {_varCnt : Countable var}
+    {_SV : SubsetEq V}
+    {_VV : VarsOf V var}
+    {_S1 : Satisfies V (A) B var}
+    {_S2 : Satisfies V ((PreTerm' symbol A)) B var}
+    {_S3 : Satisfies V (PreTerm' symbol A) (PreTerm' symbol B) var}
+    :
+    V ->
+    (PreTerm' symbol A) ->
+    Term' symbol B ->
+    Type
+:=  fun ρ a =>
+    satisfies
+    ρ (term_preterm a)
+.
+
+#[export]
+Instance Satisfies__lift_builtin_to_aosb
+    {Σ : StaticModel}
+    {V A B var : Type}
+    {_varED : EqDecision var}
+    {_varCnt : Countable var}
+    {_SV : SubsetEq V}
+    {_VV : VarsOf V var}
+    {_S1 : Satisfies V (A) B var}
+    {_S2 : Satisfies V ((PreTerm' symbol A)) B var}
+    {_S3 : Satisfies V (PreTerm' symbol A) (PreTerm' symbol B) var}
+    :
+    Satisfies
+        V
+        ((PreTerm' symbol A))
+        (Term' symbol B)
+        var
+:= {|
+    satisfies :=
+        PreTerm'_symbol_A_satisfies_SymbolicTermB' V A B var;
+|}.
+
+#[export]
+Instance Satisfies__lift_builtin_to_aosbo
+    {Σ : StaticModel}
+    {V A B var : Type}
+    {_varED : EqDecision var}
+    {_varCnt : Countable var}
+    {_SV : SubsetEq V}
+    {_VV : VarsOf V var}
+    {bsB : Satisfies V (A) B var}
+    {sat2 : Satisfies V ((PreTerm' symbol A)) B var}
+    {sat3 : Satisfies V ((PreTerm' symbol A)) (PreTerm' symbol B) var}
+    :
+    Satisfies V
+        ((Term' symbol A))
+        (Term' symbol B)
+        var
+.
+Proof. apply _. Defined.
+
+Definition PreTerm'_symbol_builtin_satisfies_SymbolicTerm
+    {Σ : StaticModel}
+    {V var : Type}
+    {_varED : EqDecision var}
+    {_varCnt : Countable var}
+    {_SV : SubsetEq V}
+    {_VV : VarsOf V var}
+    {_S1 : Satisfies V (builtin_value) BuiltinOrVar var}
+    {_S2 : Satisfies V (PreTerm' symbol builtin_value) BuiltinOrVar var}
+    {_S3 : Satisfies V (PreTerm' symbol builtin_value) (PreTerm' symbol BuiltinOrVar) var}
+    :
+    V ->
+    ((PreTerm' symbol builtin_value)) ->
+    SymbolicTerm ->
+    Type
+:=  fun ρ a =>
+    satisfies ρ (term_preterm a)
+.
+
+#[export]
+Instance Satisfies__PreTerm'_symbol_builtin__SymbolicTerm
+    {Σ : StaticModel}
+    {V var : Type}
+    {_varED : EqDecision var}
+    {_varCnt : Countable var}
+    {_SV : SubsetEq V}
+    {_VV : VarsOf V var}
+    {_S1 : Satisfies V (builtin_value) BuiltinOrVar var}
+    {_S2 : Satisfies V (PreTerm' symbol builtin_value) BuiltinOrVar var}
+    {_S3 : Satisfies V (PreTerm' symbol builtin_value) (PreTerm' symbol BuiltinOrVar) var}
+    :
+    Satisfies V
+        ((PreTerm' symbol builtin_value))
+        SymbolicTerm
+        var
+:= {|
+    satisfies :=
+        PreTerm'_symbol_builtin_satisfies_SymbolicTerm ;
+|}.
+
+
+
+
+#[local]
+Obligation Tactic := idtac.
+
+#[export]
+Instance Satisfies_builtin_expr
+    {Σ : StaticModel}:
+    Satisfies
+        Valuation
+        builtin_value
+        Expression
+        variable
+:= {|
+    satisfies := (fun ρ b e =>
+        Expression_evaluate ρ e = Some (term_operand b)
+    ) ;
+|}.
+
+
+#[export]
+Instance Satisfies_asb_expr
+    {Σ : StaticModel}:
+    Satisfies
+        Valuation
+        ((PreTerm' symbol builtin_value))
+        Expression
+        variable
+:= {|
+    satisfies := (fun ρ x e =>
+        Expression_evaluate ρ e = Some (term_preterm x)
+    ) ;
+|}.
+
+
+#[export]
+Instance Satisfies__GroundTerm__ExpressionTerm
+    {Σ : StaticModel}
+    {V var : Type}
+    {_varED : EqDecision var}
+    {_varCnt : Countable var}
+    {_SV : SubsetEq V}
+    {_VV : VarsOf V var}
+    {_S1 : Satisfies V (builtin_value) Expression var}
+    {_S2 : Satisfies V (PreTerm' symbol builtin_value) Expression var}
+    {_S3 : Satisfies V (PreTerm' symbol builtin_value) (PreTerm' symbol Expression) var}
+    :
+    Satisfies
+        V
+        GroundTerm
+        ExpressionTerm
+        var
+.
+Proof. apply _. Defined.
+
+#[export]
+Instance Satisfies_gt_var
+    {Σ : StaticModel}:
+    Satisfies
+        Valuation
+        GroundTerm
+        variable
+        variable
+:= {|
+    satisfies := (fun ρ g x => ρ !! x = Some g)
+|}.
+
+#[export]
+Instance Subseteq_ValuationLR
+    {Σ : StaticModel}
+    : SubsetEq (Valuation * LeftRight)
+:= {
+    subseteq a b := subseteq a.1 b.1 /\ a.2 = b.2
+}.
+
+
+(* TODO *)
+#[export]
+Instance VarsOf_ValuationLR
+    {Σ : StaticModel}
+    : VarsOf (Valuation * LeftRight) variable
+:= {
+    vars_of a := vars_of a.1
+}.
+
+
+#[export]
+Instance Satisfies_sym_bov
+    {Σ : StaticModel}
+    :
+    Satisfies
+        Valuation
+        symbol
+        BuiltinOrVar
+        variable
+:= {|
+    satisfies := fun _ _ _ => False ;
+|}.
+
+
+#[export]
+Instance Satisfies_Valuation_LR_SideCondition
+    {Σ : StaticModel}
+    :
+    Satisfies
+        (Valuation * LeftRight)
+        unit
+        SideCondition
+        variable
+:= {|
+    satisfies := fun ρd => let ρ := ρd.1 in
+        satisfies ρ
+        ;
+|}.
+
+Definition GroundTerm_satisfies_SymbolicTerm
+    {Σ : StaticModel}
+    : GroundTerm -> SymbolicTerm -> Type :=
+    fun g φ => { ρ : Valuation & satisfies ρ g φ }
+.
+
+#[export]
+Instance VarsOf_unit {Σ : StaticModel}: VarsOf unit variable := {|
+    vars_of _ := ∅ ;
+|}.
+
+#[export]
+Instance Subseteq_unit {Σ : StaticModel}: SubsetEq unit := 
+    fun _ _ => true
+.
+
+
+#[export]
+Instance Satisfies__GroundTerm__SymbolicTerm_inall
+    {Σ : StaticModel}
+    :
+    Satisfies
+        unit
+        GroundTerm
+        SymbolicTerm
+        variable
+:= {|
+    satisfies := fun _ => GroundTerm_satisfies_SymbolicTerm ;
+|}.
+
+#[export]
+Instance Satisfies_valuation_scs
+    {Σ : StaticModel}
+    : Satisfies
+        Valuation
+        unit
+        (list SideCondition)
+        variable
+:= {|
+    satisfies := fun ρ _ l => forall x, x ∈ l -> satisfies ρ () x;
+|}.
+
+#[export]
+Instance
+    Satisfies_symbol_B
+    {Σ : StaticModel}
+    {V B var : Type}
+    {_SV : SubsetEq V}
+    {_EDvar : EqDecision var}
+    {_Covar : Countable var}
+    {_VV : VarsOf V var}
+    :
+    Satisfies
+        V
+        symbol
+        B
+        var
+:= {|
+    satisfies := fun _ _ _ => False ;
+|}.
+
+Definition flattened_rewrites_in_valuation_under_to
+    {Σ : StaticModel}
+    {Act : Set}
+    (ρ : Valuation)
+    (r : RewritingRule Act)
+    (from : GroundTerm)
+    (under : Act)
+    (to : GroundTerm)
+    : Type
+:= ((satisfies ρ from (fr_from r))
+* (satisfies ρ to (fr_to r))
+* (@satisfies Σ Valuation unit (list SideCondition) _ _ _ _ _ _ ρ tt (fr_scs r))
+* (under = fr_act r)
+)%type
+.
+
+
+Definition flattened_rewrites_to
+    {Σ : StaticModel}
+    {Act : Set}
+    (r : RewritingRule Act)
+    (from : GroundTerm)
+    (under : Act)
+    (to : GroundTerm)
+    : Type
+:= { ρ : Valuation &
+    flattened_rewrites_in_valuation_under_to ρ r from under to
+   }
+.
+
+
+
+
+#[export]
+Instance Satisfies_TermOverBuiltin_TermOverBoV
+    {Σ : StaticModel}
+    : Satisfies
+        Valuation
+        (TermOver builtin_value)
+        (TermOver BuiltinOrVar)
+        variable
+:= {|
+    satisfies := fun ρ tg ts => satisfies ρ (uglify' tg) (uglify' ts) ;
+|}.
+
+
+
+#[export]
+Instance Satisfies_TermOverBuiltin_TermOverExpression
+    {Σ : StaticModel}
+    : Satisfies
+        Valuation
+        (TermOver builtin_value)
+        (TermOver Expression)
+        variable
+:= {|
+    satisfies := fun ρ tg ts => satisfies ρ (uglify' tg) (uglify' ts) ;
+|}.
+
+
+
+Inductive flattened_rewrites_to_over
+    {Σ : StaticModel}
+    {Act : Set}
+    (Γ : RewritingTheory Act)
+    :
+    TermOver builtin_value ->
+    list Act ->
+    TermOver builtin_value ->
+    Type
+:=
+| frto_base: forall t,
+        flattened_rewrites_to_over Γ t nil t
+| frto_step: forall (t1 t2 t3 : TermOver builtin_value) w a r,
+    r ∈ Γ ->
+    flattened_rewrites_to r (uglify' t1) a (uglify' t2) ->
+    flattened_rewrites_to_over Γ t2 w t3 ->
+    flattened_rewrites_to_over Γ t1 (a::w) t3
+.
+
