minuska/theories/minusl_syntax.v
@@ -2,7 +2,8 @@ From stdpp Require Import finite.
 
 From Minuska Require Import
     prelude
-    spec_syntax
+    spec
+    lowlang
     syntax_properties
     varsof
 .
