minuska/theories/semantics_properties.v
@@ -1,9 +1,10 @@
 From Minuska Require Import
     prelude
-    spec_syntax
-    spec_semantics
+    spec
+    lowlang
     varsof
     syntax_properties
+    properties
 .
 
 Lemma Expression_evaluate_extensive_Some
