minuska/theories/spec.v
@@ -1,0 +1,626 @@
+From Minuska Require Import
+    prelude
+.
+
+From Equations Require Export Equations.
+
+
+(*
+    Here we define an alternative, more user-friendly term structure.
+*)
+
+Unset Elimination Schemes.
+#[universes(polymorphic=yes, cumulative=yes)]
+Inductive TermOver' {T : Type} (A : Type) : Type :=
+| t_over (a : A)
+| t_term (s : T) (l : list (@TermOver' T A))
+.
+Set Elimination Schemes.
+
+Arguments t_over {T} {A}%_type_scope a.
+Arguments t_term {T} {A}%_type_scope s l%_list_scope.
+
+Section custom_induction_principle.
+
+    Context
+        {T : Type}
+        {A : Type}
+        (P : @TermOver' T A -> Prop)
+        (true_for_over : forall a, P (t_over a) )
+        (preserved_by_term :
+            forall
+                (s : T)
+                (l : list (@TermOver' T A)),
+                Forall P l ->
+                P (t_term s l)
+        )
+    .
+
+    Fixpoint TermOver'_ind (p : @TermOver' T A) : P p :=
+    match p with
+    | t_over a => true_for_over a
+    | t_term s l => preserved_by_term s l (Forall_true P l TermOver'_ind)
+    end.
+
+End custom_induction_principle.
+
+Class MVariables (variable : Type) := {
+    variable_eqdec :: EqDecision variable ;
+    variable_countable :: Countable variable ;
+    variable_infinite :: Infinite variable ;
+}.
+
+Class Symbols (symbol : Type) := {
+    symbol_eqdec :: EqDecision symbol ;
+    symbol_countable :: Countable symbol ;
+}.
+
+Class Builtin {symbol : Type} {symbols : Symbols symbol} := {
+    builtin_value
+        : Type ;
+    builtin_value_eqdec
+        :: EqDecision builtin_value ;
+    
+    builtin_nullary_function
+        : Type ;
+    builtin_nullary_function_eqdec
+        :: EqDecision builtin_nullary_function ;
+
+    builtin_unary_function
+        : Type ;
+    builtin_unary_function_eqdec
+        :: EqDecision builtin_unary_function ;
+
+    builtin_binary_function
+        : Type ;
+    builtin_binary_function_eqdec
+        :: EqDecision builtin_binary_function ;
+    
+    builtin_ternary_function
+        : Type ;
+    builtin_ternary_function_eqdec
+        :: EqDecision builtin_ternary_function ;
+
+    builtin_nullary_function_interp
+        : builtin_nullary_function
+        -> (@TermOver' symbol builtin_value) ;
+
+    builtin_unary_function_interp
+        : builtin_unary_function
+        -> (@TermOver' symbol builtin_value)
+        -> (@TermOver' symbol builtin_value) ;
+
+    builtin_binary_function_interp
+        : builtin_binary_function
+        -> (@TermOver' symbol builtin_value)
+        -> (@TermOver' symbol builtin_value)
+        -> (@TermOver' symbol builtin_value) ;
+
+    builtin_ternary_function_interp
+        : builtin_ternary_function
+        -> (@TermOver' symbol builtin_value)
+        -> (@TermOver' symbol builtin_value)
+        -> (@TermOver' symbol builtin_value)
+        -> (@TermOver' symbol builtin_value) ;
+}.
+
+Class StaticModel := {
+    symbol : Type ;
+    variable : Type ;
+    symbols :: Symbols symbol ;
+    builtin :: Builtin ;
+    variables :: MVariables variable ;
+}.
+
+Class VarsOf
+    (A : Type)
+    (var: Type)
+    {_Ev : EqDecision var}
+    {_Cv : Countable var}
+    :=
+{
+    vars_of : A -> gset var ;
+}.
+
+Arguments vars_of : simpl never.
+
+
+Inductive Expression2
+    {Σ : StaticModel}
+    :=
+| e_ground (e : @TermOver' (symbol) builtin_value)
+| e_variable (x : variable)
+| e_nullary (f : builtin_nullary_function)
+| e_unary (f : builtin_unary_function) (t : Expression2)
+| e_binary (f : builtin_binary_function) (t1 : Expression2) (t2 : Expression2)
+| e_ternary (f : builtin_ternary_function) (t1 : Expression2) (t2 : Expression2) (t3 : Expression2)
+.
+
+
+Inductive BuiltinOrVar {Σ : StaticModel} :=
+| bov_builtin (b : builtin_value)
+| bov_variable (x : variable)
+.
+
+
+
+
+Definition TermOver {Σ : StaticModel} (A : Type) : Type := @TermOver' symbol A.
+
+Fixpoint TermOver_size
+    {T : Type}
+    {A : Type}
+    (t : @TermOver' T A)
+    : nat
+:=
+match t with
+| t_over _ => 1
+| t_term _ l => S (sum_list_with (S ∘ TermOver_size) l)
+end.
+
+Fixpoint vars_of_to_l2r
+    {Σ : StaticModel}
+    (t : TermOver BuiltinOrVar)
+    : list variable
+:= 
+    match t with
+    | t_over (bov_builtin _) => []
+    | t_over (bov_variable x) => [x]
+    | t_term s l => concat (map vars_of_to_l2r l)
+    end
+.
+
+
+Fixpoint TermOverBoV_subst
+    {Σ : StaticModel}
+    (t : TermOver BuiltinOrVar)
+    (x : variable)
+    (t' : TermOver BuiltinOrVar)
+:=
+match t with
+| t_over (bov_builtin b) => t_over (bov_builtin b)
+| t_over (bov_variable y) =>
+    match (decide (x = y)) with
+    | left _ => t'
+    | right _ => t_over (bov_variable y)
+    end
+| t_term s l => t_term s (map (fun t'' => TermOverBoV_subst t'' x t') l)
+end.
+
+Fixpoint TermOver_map
+    {Σ : StaticModel}
+    {A B : Type}
+    (f : A -> B)
+    (t : TermOver A)
+    : TermOver B
+:=
+    match t with
+    | t_over b => t_over (f b)
+    | t_term s l => t_term s (map (TermOver_map f) l)
+    end
+.
+
+Definition TermOverBuiltin_to_TermOverBoV
+    {Σ : StaticModel}
+    (t : TermOver builtin_value)
+    : TermOver BuiltinOrVar
+:=
+    TermOver_map bov_builtin t
+.
+
+
+
+
+Fixpoint Expression2_subst
+    {Σ : StaticModel}
+    (e : Expression2)
+    (x : variable)
+    (e' : Expression2)
+    : Expression2
+:=    
+match e with
+| e_ground g => e_ground g
+| e_variable y =>
+    if (decide (y = x)) then e' else (e_variable y)
+| e_nullary f => e_nullary f
+| e_unary f e1 => e_unary f (Expression2_subst e1 x e')
+| e_binary f e1 e2 => e_binary f (Expression2_subst e1 x e') (Expression2_subst e2 x e')
+| e_ternary f e1 e2 e3 => e_ternary f (Expression2_subst e1 x e') (Expression2_subst e2 x e') (Expression2_subst e3 x e')
+end
+.
+
+Record SideCondition2
+    {Σ : StaticModel}
+    :=
+mkSideCondition2 {
+    sc_left: Expression2 ;
+    sc_right: Expression2 ;
+}.
+
+
+Record RewritingRule2
+    {Σ : StaticModel}
+    (Act : Set)
+:= mkRewritingRule2
+{
+    r_from : TermOver BuiltinOrVar ;
+    r_to : TermOver Expression2 ;
+    r_scs : list SideCondition2 ;
+    r_act : Act ;
+}.
+
+Arguments r_from {Σ} {Act%_type_scope} r.
+Arguments r_to {Σ} {Act%_type_scope} r.
+Arguments r_scs {Σ} {Act%_type_scope} r.
+Arguments r_act {Σ} {Act%_type_scope} r.
+
+
+
+Definition RewritingTheory2
+    {Σ : StaticModel}
+    (Act : Set)
+    := list (RewritingRule2 Act)
+.
+
+
+Fixpoint vars_of_Expression2
+    {Σ : StaticModel}
+    (t : Expression2)
+    : gset variable :=
+match t with
+| e_ground _ => ∅
+| e_variable x => {[x]}
+| e_nullary _ => ∅
+| e_unary _ t' => vars_of_Expression2 t'
+| e_binary _ t1 t2 => vars_of_Expression2 t1 ∪ vars_of_Expression2 t2
+| e_ternary _ t1 t2 t3 => vars_of_Expression2 t1 ∪ vars_of_Expression2 t2 ∪ vars_of_Expression2 t3
+end.
+
+#[export]
+Instance VarsOf_Expression2
+    {Σ : StaticModel}
+    : VarsOf Expression2 variable
+:= {|
+    vars_of := vars_of_Expression2 ; 
+|}.
+
+
+
+#[export]
+Instance VarsOf_symbol
+    {Σ : StaticModel}
+    : VarsOf symbol variable
+:= {|
+    vars_of := fun _ => ∅ ; 
+|}.
+
+#[export]
+Instance VarsOf_builtin
+    {Σ : StaticModel}
+    : VarsOf builtin_value variable
+:= {|
+    vars_of := fun _ => ∅ ; 
+|}.
+
+
+#[export]
+Instance VarsOf_SideCondition2
+    {Σ : StaticModel}
+    : VarsOf SideCondition2 variable
+:= {|
+    vars_of := fun c => vars_of (sc_left c) ∪ vars_of (sc_right c) ; 
+|}.
+
+#[export]
+Program Instance VarsOf_list_SideCondition2
+    {Σ : StaticModel}
+    : VarsOf (list SideCondition2) variable
+:= {|
+    vars_of := fun scs => ⋃ (vars_of <$> scs)
+|}.
+
+
+
+Class Satisfies
+    {Σ : StaticModel}
+    (V A B var : Type)
+    {_SV : SubsetEq V}
+    {_varED : EqDecision var}
+    {_varCnt : Countable var}
+    {_VV: VarsOf V var}
+    :=
+mkSatisfies {
+    satisfies :
+        V -> A -> B -> Type ;
+}.
+
+Arguments satisfies : simpl never.
+
+
+Definition Valuation2
+    {Σ : StaticModel}
+:=
+    gmap variable (TermOver builtin_value)
+.
+
+
+#[export]
+Instance Subseteq_Valuation2 {Σ : StaticModel}
+    : SubsetEq Valuation2
+.
+Proof.
+    unfold Valuation2.
+    apply _.
+Defined.
+
+#[export]
+Instance VarsOf_Valuation2_
+    {Σ : StaticModel}
+    {var : Type}
+    {_varED : EqDecision var}
+    {_varCnt : Countable var}
+    : VarsOf (gmap var (TermOver BuiltinOrVar)) var
+:= {|
+    vars_of := fun ρ => dom ρ ; 
+|}.
+
+#[export]
+Instance VarsOf_Valuation2
+    {Σ : StaticModel}
+    : VarsOf (Valuation2) variable
+:= {|
+    vars_of := fun ρ => dom ρ ; 
+|}.
+
+
+
+Definition Satisfies_Valuation2_TermOverBuiltinValue_BuiltinOrVar
+    {Σ : StaticModel}
+    (ρ : Valuation2)
+    (t : TermOver builtin_value)
+    (bv : BuiltinOrVar)
+    : Prop
+:= match bv with
+    | bov_builtin b => t = t_over b
+    | bov_variable x => ρ !! x = Some t
+    end
+.
+
+#[export]
+Instance Satisfies_Valuation2_TermOverBuiltinValue_BuiltinOrVar_instnace
+    {Σ : StaticModel}
+    : Satisfies
+        Valuation2
+        (TermOver builtin_value)
+        (BuiltinOrVar)
+        variable
+:= {|
+    satisfies := fun ρ tg ts => Satisfies_Valuation2_TermOverBuiltinValue_BuiltinOrVar ρ tg ts ;
+|}.
+
+Equations? sat2B
+    {Σ : StaticModel}
+    (ρ : Valuation2)
+    (t : TermOver builtin_value)
+    (φ : TermOver BuiltinOrVar)
+    : Prop
+    by wf (TermOver_size φ) lt
+:=
+    sat2B ρ t (t_over bv) := Satisfies_Valuation2_TermOverBuiltinValue_BuiltinOrVar ρ t bv ;
+    sat2B ρ (t_over _) (t_term s l) := False ;
+    sat2B ρ (t_term s' l') (t_term s l) :=
+        ((s' = s) /\
+        (length l' = length l) /\
+        forall i t' φ' (pf1 : l !! i = Some φ') (pf2 : l' !! i = Some t'),
+            sat2B ρ t' φ'
+        )
+    ;
+.
+Proof.
+    abstract(
+    unfold satisfies in *; simpl in *;
+    simpl;
+    apply take_drop_middle in pf1;
+    rewrite <- pf1;
+    rewrite sum_list_with_app; simpl;
+    ltac1:(lia)).
+Defined.
+
+
+
+Fixpoint Expression2_evaluate
+    {Σ : StaticModel}
+    (ρ : Valuation2)
+    (t : Expression2)
+    : option (TermOver builtin_value) :=
+match t with
+| e_ground e => Some e
+| e_variable x => ρ !! x
+| e_nullary f =>
+    Some ((builtin_nullary_function_interp f))
+| e_unary f t =>
+    e ← Expression2_evaluate ρ t;
+    Some ((builtin_unary_function_interp f (e)))
+| e_binary f t1 t2 =>
+    e1 ← Expression2_evaluate ρ t1;
+    e2 ← Expression2_evaluate ρ t2;
+    Some ((builtin_binary_function_interp f (e1) (e2)))
+| e_ternary f t1 t2 t3 =>
+    e1 ← Expression2_evaluate ρ t1;
+    e2 ← Expression2_evaluate ρ t2;
+    e3 ← Expression2_evaluate ρ t3;
+    Some ((builtin_ternary_function_interp f (e1) (e2) (e3)))
+end.
+
+
+
+
+Equations? sat2E
+    {Σ : StaticModel}
+    (ρ : Valuation2)
+    (t : TermOver builtin_value)
+    (φ : TermOver Expression2)
+    : Prop
+    by wf (TermOver_size φ) lt
+:=
+    sat2E ρ t (t_over e) := Expression2_evaluate ρ e = Some t;
+    sat2E ρ (t_over a) (t_term s l) := False ;
+    sat2E ρ (t_term s' l') (t_term s l) :=
+        s' = s /\
+        length l' = length l /\
+        forall i t' φ' (pf1 : l !! i = Some φ') (pf2 : l' !! i = Some t'),
+            sat2E ρ t' φ'
+    ;
+.
+Proof.
+    abstract(
+        simpl;
+        apply take_drop_middle in pf1;
+        rewrite <- pf1;
+        rewrite sum_list_with_app; simpl;
+        ltac1:(lia)
+    ).
+Defined.
+
+
+#[export]
+Instance Satisfies_TermOverBuiltin_TermOverExpression2
+    {Σ : StaticModel}
+    : Satisfies
+        Valuation2
+        (TermOver builtin_value)
+        (TermOver Expression2)
+        variable
+:= {|
+    satisfies := fun ρ tg ts => sat2E ρ tg ts ;
+|}.
+
+#[export]
+Instance Satisfies_SideCondition2
+    {Σ : StaticModel}
+    : Satisfies
+        Valuation2
+        unit
+        SideCondition2
+        variable
+:= {|
+    satisfies := fun ρ _ sc =>
+        Expression2_evaluate ρ (sc_left sc) = 
+        Expression2_evaluate ρ (sc_right sc) /\
+        isSome (Expression2_evaluate ρ (sc_left sc));
+|}.
+
+
+#[export]
+Instance Satisfies_Valuation2_scs2
+    {Σ : StaticModel}
+    : Satisfies
+        Valuation2
+        unit
+        (list SideCondition2)
+        variable
+:= {|
+    satisfies := fun ρ _ l => forall x, x ∈ l -> satisfies ρ () x;
+|}.
+
+
+
+#[export]
+Instance VarsOf_TermOver
+    {T0 : Type}
+    {T var : Type}
+    {_EDv : EqDecision var}
+    {_Cv : Countable var}
+    {_VT : VarsOf T var}
+    :
+    VarsOf (@TermOver' T0 T) var
+:=
+{|
+    vars_of := (fix go (t : @TermOver' T0 T) := 
+        match t with
+        | t_over x => vars_of x
+        | t_term _ l => ⋃ (go <$> l)
+        end
+    ) ; 
+|}.
+
+Definition vars_of_BoV
+    {Σ : StaticModel}
+    (bov : BuiltinOrVar)
+    : gset variable
+:=
+match bov with
+| bov_variable x => {[x]}
+| bov_builtin _ => ∅
+end.
+
+#[export]
+Instance VarsOf_BoV
+    {Σ : StaticModel}
+    : VarsOf BuiltinOrVar variable
+:= {|
+    vars_of := vars_of_BoV ; 
+|}.
+
+
+#[export]
+Instance VarsOf_TermOver_BuiltinOrVar
+    {Σ : StaticModel}
+    :
+    VarsOf (TermOver BuiltinOrVar) variable
+.
+Proof.
+    apply VarsOf_TermOver.
+Defined.
+
+#[export]
+Instance VarsOf_TermOver_Expression2
+    {Σ : StaticModel}
+    :
+    VarsOf (TermOver Expression2) variable
+.
+Proof.
+    apply VarsOf_TermOver.
+Defined.
+
+
+#[export]
+Instance Satisfies_Valuation2_TermOverBuiltin_TermOverBoV
+    {Σ : StaticModel}
+    : Satisfies
+        Valuation2
+        (TermOver builtin_value)
+        (TermOver BuiltinOrVar)
+        variable
+:= {|
+    satisfies := fun ρ tg ts => sat2B ρ tg ts
+|}.
+
+Definition rewrites_in_valuation_under_to
+    {Σ : StaticModel}
+    {Act : Set}
+    (ρ : Valuation2)
+    (r : RewritingRule2 Act)
+    (from : TermOver builtin_value)
+    (under : Act)
+    (to : TermOver builtin_value)
+    : Type
+:= ((@satisfies Σ Valuation2 (TermOver builtin_value) (TermOver BuiltinOrVar) (@variable Σ) _ _ _ _ _ ρ from (r_from r))
+* (@satisfies Σ Valuation2 (TermOver builtin_value) (TermOver Expression2) (@variable Σ) _ _ _ _ _ ρ to (r_to r))
+* (@satisfies Σ Valuation2 unit (list SideCondition2) (@variable Σ) _ _ _ _ _ ρ tt (r_scs r))
+* (under = r_act r)
+)%type
+.
+
+Definition rewrites_to
+    {Σ : StaticModel}
+    {Act : Set}
+    (r : RewritingRule2 Act)
+    (from : TermOver builtin_value)
+    (under : Act)
+    (to : TermOver builtin_value)
+    : Type
+:= { ρ : Valuation2 &
+    rewrites_in_valuation_under_to ρ r from under to
+   }
+.
