minuska/theories/spec_lowlang_interpreter.v
@@ -1,0 +1,135 @@
+From Minuska Require Import
+    prelude
+    spec
+    lowlang
+    varsof
+    syntax_properties
+.
+
+
+
+Definition RewritingRule_wf1
+    {Σ : StaticModel}
+    {Act : Set}
+    (r : RewritingRule Act)
+    : Type
+:= 
+    let vs1 : gset variable := vars_of (fr_scs r) in
+    let vs2 : gset variable := vars_of (fr_from r) in
+    (vs1 ⊆ vs2)
+.
+
+Definition RewritingRule_wf2'
+    {Σ : StaticModel}
+    {Act : Set}
+    (r : RewritingRule Act)
+    : Type
+:= 
+    (vars_of (fr_to r) ⊆ vars_of (fr_from r))
+.
+
+
+(*
+    This is known as 'weakly well-defined rule'
+    in the literature.
+*)
+Definition RewritingRule_wf2
+    {Σ : StaticModel}
+    {Act : Set}
+    (r : RewritingRule Act)
+    : Type
+:= 
+    forall (g : GroundTerm) (ρ : Valuation),
+        satisfies ρ g (fr_from r) ->
+        satisfies ρ () (fr_scs r) ->
+        { g' : GroundTerm &
+            satisfies ρ g' (fr_to r)
+        }
+.
+
+Definition RewritingRule_wf
+    {Σ : StaticModel}
+    {Act : Set}
+    (r : RewritingRule Act)
+    : Type
+:=
+    RewritingRule_wf1 r * RewritingRule_wf2 r
+.
+
+Definition RewritingTheory_wf
+    {Σ : StaticModel}
+    {Act : Set}
+    (Γ : RewritingTheory Act)
+    : Type
+:=
+    forall r, r ∈ Γ -> RewritingRule_wf r
+.
+
+Definition rewriting_relation_flat
+    {Σ : StaticModel}
+    {Act : Set}
+    (Γ : list (RewritingRule Act))
+    : GroundTerm -> GroundTerm -> Type
+    := fun from to =>
+        { r : _ & { a : _ & ((r ∈ Γ) * flattened_rewrites_to r from a to)%type}}
+.
+
+
+Definition not_stuck_flat
+    {Σ : StaticModel}
+    {Act : Set}
+    (Γ : list (RewritingRule Act))
+    (e : GroundTerm) : Type
+:=
+    { e' : _ & rewriting_relation_flat Γ e e' }
+.
+
+Definition flat_stuck
+    {Σ : StaticModel}
+    {Act : Set}
+    (Γ : list (RewritingRule Act))
+    (e : GroundTerm) : Type
+:=
+    notT (not_stuck_flat Γ e)
+.
+
+
+Definition FlatInterpreter
+    {Σ : StaticModel}
+    {Act : Set}
+    (Γ : list (RewritingRule Act))
+    : Type
+    := GroundTerm -> option GroundTerm
+.
+
+Definition FlatInterpreter_sound'
+    {Σ : StaticModel}
+    {Act : Set}
+    (Γ : list (RewritingRule Act))
+    (interpreter : FlatInterpreter Γ)
+    : Type
+    := ((
+        forall e1 e2,
+            interpreter e1 = Some e2 ->
+            rewriting_relation_flat Γ e1 e2
+    )
+    *
+    (forall e,
+        flat_stuck Γ e -> interpreter e = None)
+    * (forall e,
+        not_stuck_flat Γ e ->
+        exists e', interpreter e = Some e')
+    )%type
+.
+
+
+Definition FlatInterpreter_sound
+    {Σ : StaticModel}
+    {Act : Set}
+    (Γ : list (RewritingRule Act))
+    (interpreter : FlatInterpreter Γ)
+    : Type
+:= 
+    RewritingTheory_wf Γ ->
+    FlatInterpreter_sound' Γ interpreter
+.
