minuska/theories/try_match.v
@@ -1,8 +1,9 @@
 From Minuska Require Import
     prelude
-    spec_syntax
-    spec_semantics
+    spec
+    lowlang
     syntax_properties
+    properties
     semantics_properties
     basic_matching
 .
